generic version of base_w procedure

spec/Correctness_WOTS.ec
@@ -1,4 +1,72 @@
+require import AllCore List RealExp IntDiv.
+require Subtype. 
+
+from Jasmin require import JModel.
+
+require import Notation Parameters Address Primitives Wots.
+
+import NBytes.
+import Array8.
+
+require import XMSS_IMPL.
+
 (*
     We first prove that the equivalence between the extracted EC and the preprocessed EC
     We then prove that the preprocessed EC is equivalent to the specification (so the extracted EC is also equivalent to the spec)
 *)
+
+require import Array2 Array3.
+
+module BaseWGeneric = {
+proc __base_w (output : W32.t list, input : W8.t list) : W32.t list = {
+
+    var in_0:W64.t;
+    var out:W64.t;
+    var bits:W64.t;
+    var consumed:W64.t;
+    var total:W8.t <- witness;
+    var total_32:W32.t;
+    var _of_:bool;
+    var _cf_:bool;
+    var _sf_:bool;
+    var _zf_:bool;
+    var  _0:bool;
+
+    var inlen : W64.t <- W64.of_int (size input);
+    var outlen : W64.t <- W64.of_int (size output);
+
+    in_0 <- W64.zero;
+    out <- W64.zero;
+    bits <- W64.zero;
+    consumed <-W64.zero;
+
+    while ((consumed \ult outlen)) {
+      if (bits = W64.zero) {
+        total <- input.[(W64.to_uint in_0)];
+        in_0 <- (in_0 + (W64.of_int 1));
+        bits <- (bits + (W64.of_int 8));
+      }
+      
+      bits <- (bits - (W64.of_int 4));
+      total_32 <- (zeroextu32 total);
+      (_of_, _cf_, _sf_,  _0, _zf_, total_32) <- SHR_32 total_32 (truncateu8 bits);
+      total_32 <- (total_32 `&` (W32.of_int (16 - 1)));
+      output <- put output (W64.to_uint out) total_32; (* output.[(W64.to_uint out)] <- total_32; *)
+      out <- (out + (W64.of_int 1));
+      consumed <- (consumed + (W64.of_int 1));
+    }
+
+    return (output);
+  }
+}.
+
+lemma base_w_generic_1 (output : W32.t Array3.t, input : W8.t Array2.t):
+    equiv[M(Syscall).__base_w_3_2 ~ BaseWGeneric.__base_w :
+       arg{1} = (output, input) /\
+       arg{2} = (mkseq (fun i => output.[i]) 3, 
+                 mkseq (fun i => input.[i]) 2) ==> 
+      mkseq (fun i => res{1}.[i]) 3 = res{2}].
+proc.
+auto => /> *.
+admit.
+qed.
