spec/Utils.ec
@@ -1,0 +1,10 @@
+pragma Goals : printall.
+
+require import AllCore List RealExp IntDiv.
+require import WArray32.
+
+from Jasmin require import JModel_x86.
+
+require import XMSS_IMPL.
+
+(* Lemma __u32_to_bytes *)
