spec/XMSS.ec
@@ -8,8 +8,6 @@ require import Notation Parameters Address Primitives Wots.
 import NBytes.
 import Array8.
 
-(**********************************************************************************************************************)
-
 clone import Subtype as Bitmask with 
    type T = byte list,
    op P = fun l => size l = 2 * n
@@ -24,40 +22,36 @@ clone import Subtype as Three_NBytes with
    proof inhabited by (exists (nseq (3*n) W8.zero);smt(size_nseq ge0_n))
    proof *.
 
-clone import Subtype as SIG_OTS with 
-   type T = nbytes list,
-   op P = fun l => size l = len
-   rename "T" as "sig_ots"
-   proof inhabited by admit.
-
-(**********************************************************************************************************************)
-
-op remove_last (x : 'a list) : 'a list = 
-with x = [] => []
-with x = h::t => if t = [] then [] else remove_last t.
-
-abbrev push (x : 'a list) (a : 'a) : 'a list = rcons x a. 
-abbrev pop (x : 'a list) : 'a list * 'a = 
-    let last_elem : 'a = last witness x in
-    let new_list = remove_last x in
-    (new_list, last_elem).
-
-(**********************************************************************************************************************)
+(*********************************************************************************************)
 
 op h : { int | 0 < h } as h.
 op max_signatures : int = 2^h.
 
+(*
+Besides the cryptographic hash function F and the pseudorandom
+function PRF required by WOTS+, XMSS uses two more functions:
+
+-  A cryptographic hash function H.  H accepts n-byte keys and byte
+      strings of length 2n and returns an n-byte string.
+
+-  A cryptographic hash function H_msg.  H_msg accepts 3n-byte keys
+      and byte strings of arbitrary length and returns an n-byte string.
+ *)
 op H : nbytes -> bitmask -> nbytes.
 op H_msg : tree_n_bytes -> byte list -> nbytes.
 
-op oid : W32.t.
-op zero_address : adrs = Array8.init (fun _ => W32.zero).
+type oid =  W32.t.
 
 (* Format sk: [OID || (ceil(h/8) bit) idx || SK_SEED || SK_PRF || PUB_SEED || root] *)
-type sk_t = W32.t * W32.t * nbytes * nbytes * nbytes * nbytes.
+type sk_t = oid * W32.t * nbytes * nbytes * nbytes * nbytes.
+
+(* Format pk: [OID || root || PUB_SEED] *)
+type pk_t = oid * nbytes * nbytes.
+
+type keypair = pk_t * sk_t.
 
 (*
-(* Format pk: [OID || root || PUB_SEED] *)
+
             +---------------------------------+
             |          algorithm OID          |
             +---------------------------------+
@@ -72,85 +66,36 @@ type sk_t = W32.t * W32.t * nbytes * nbytes * nbytes * nbytes.
 
                               XMSS Public Key
 *)
-type pk_t = W32.t * nbytes * nbytes.
 
-type keypair = pk_t * sk_t.
+(**********************************************************************************************)
 
-
-(*
-             +---------------------------------+
-             |                                 |
-             |          index idx_sig          |    4 bytes
-             |                                 |
-             +---------------------------------+
-             |                                 |
-             |          randomness r           |    n bytes
-             |                                 |
-             +---------------------------------+
-             |                                 |
-             |     WOTS+ signature sig_ots     |    len * n bytes
-             |                                 |
-             +---------------------------------+
-             |                                 |
-             |             auth[0]             |    n bytes
-             |                                 |
-             +---------------------------------+
-             |                                 |
-             ~              ....               ~
-             |                                 |
-             +---------------------------------+
-             |                                 |
-             |           auth[h - 1]           |    n bytes
-             |                                 |
-             +---------------------------------+
-
-                        XMSS Signature
-*)
-type sig_t = W32.t * nbytes * sig_ots * nbytes list.
-
-type msg_t = byte list.
-
-(**********************************************************************************************************************)
-
-type authentication_path = nbytes list.
-op build_authpath : authentication_path.
-
-(**********************************************************************************************************************)
-
-op get_sk_seed (sk : sk_t) : nbytes = sk.`3.
-op get_seed (sk : sk_t) : nbytes = sk.`5. (* This is the pub seed *)
-
-(**********************************************************************************************************************)
-
+(* 4.1.4 Randomized tree hashing *)
 op rand_hash (_left _right : nbytes, _seed : seed, address : adrs) : nbytes = 
   let address : adrs = set_key_and_mask address 0 in
-  let key : nbytes = prf _seed address in
+  let key : nbytes = PRF _seed address in
   let address : adrs = set_key_and_mask address 1 in
-  let bitmask_0 : nbytes = prf _seed address in
+  let bitmask_0 : nbytes = PRF _seed address in
   let address : adrs = set_key_and_mask address 2 in
-  let bitmask_1 : nbytes = prf _seed address in
+  let bitmask_1 : nbytes = PRF _seed address in
   let hash_in : nbytes = (nbytexor _left bitmask_0) ++ (nbytexor _right bitmask_1) in
   H key hash_in.
 
-(**********************************************************************************************************************)
+(**************************************************************************************************)
 
-abbrev (>) (a b : int) = b < a. 
-
+(* 4.1.5 L-Trees *)
 module LTree = {
   proc ltree (pk : wots_pk, address : adrs, _seed : seed) : nbytes = {
     var _len : int <- len;
     var pk_i : nbytes;
     var tmp : nbytes;
-    var i : int;
-
-    i <- witness; (* suppress warning *)
+    var i : int <- witness;
 
     address <- set_tree_height address 0;
 
     while (_len > 1) {
       i <- 0;
       while (i < floor (len%r / 2%r)) {
-        address <-set_tree_index address i;
+        address <- set_tree_index address i;
         pk_i <- nth witness pk (2*i);
         tmp <- nth witness pk (2*i + 1);
         pk_i <- rand_hash pk_i tmp _seed address;
@@ -169,142 +114,35 @@ module LTree = {
 
     return pk_i;
   }
-}.
+}. 
 
-(**********************************************************************************************************************)
+(**************************************************************************************************)
+
+(* Stack operations *)
+abbrev push (x : 'a list) (a : 'a) : 'a list = rcons x a. 
+
+(* TODO: Replace with belast ? *)
+op remove_last (x : 'a list) : 'a list = 
+with x = [] => []
+with x = h::t => if t = [] then [] else remove_last t.
+
+abbrev pop (x : 'a list) : 'a list * 'a = 
+    let last_elem : 'a = last witness x in
+    let new_list = remove_last x in
+    (new_list, last_elem).
 
 (* It is REQUIRED that s % 2^t = 0, i.e., that the leaf at index s is a leftmost leaf of a sub-tree of height t. *)
 pred leftmost_leaf (s t : int)  = s %% 2^t = 0.
 
 pred treehash_p (s t : int) = s %% (1 `<<` t) <> 0.
 
-op same_height : nbytes -> int -> bool.
+op same_height : nbytes -> int -> bool. (* TODO: *)
 
-module Treehash = {
-  proc treehash(sk : sk_t, s t : int, address : adrs) : nbytes = {
-    var stack : nbytes list;
-    var node : nbytes;
-    var top_node : nbytes;
-    var _seed : seed;
-    var pk : wots_pk;
-    var i : int <- 0;
-    var tree_index, tree_height: int;
 
-    pk <- witness; (* To suppress warning *)
-    stack <- witness;
-
-    while (i < 2^t) {
-      _seed  <- get_seed sk;
-      address <- set_type address 0;
-      address <- set_ots_addr address (s + 1);
-      (*123*)
-      (* pk <- genPKWots pk sk _seed address; *)
-      address <- set_type address 1;
-      address <- set_tree_addr address (s + 1);
-      node <@ LTree.ltree(pk, address, _seed); 
-      address <- set_type address 2;
-      address <- set_tree_height address 0;
-      address <- set_tree_index address (i + 1);
-      
-      top_node <- last witness stack;
-      while (same_height top_node t) {
-        tree_index <- get_tree_index address;
-        address <- set_tree_index address (ceil((tree_index - 1)%r / 2%r));
-        (stack, top_node) <- pop stack;
-        node <- rand_hash top_node node _seed address;
-        
-        tree_height <- get_tree_height address;
-        address <- set_tree_height address (tree_height + 1);
-      }
-      stack <- push stack node;
-
-    }
-
-    (stack, node) <- pop stack;
-    return node;
-  }
-}.
-
-(**********************************************************************************************************************)
-
-module AuthPath = {
-  proc buildAuth(sk : sk_t, index : int, address : adrs) : authentication_path = {
-    var authpath : authentication_path <- witness;
-    var j : int <- 0;
-    
-    while (j < h) {
-      j <- j+1;
-    }
-
-    return authpath;
-  }
-}.
-
-op treeSig (m : nbytes, sk : sk_t, index : W32.t, address : adrs) =
-  let authpath : authentication_path = witness (* AuthPath.buildAuth(sk, W32.to_uint index, address) *) in
-  let address : adrs = set_type address 0 in
-  let address : adrs = set_ots_addr address (W32.to_uint index) in
-  let sig_ots = witness in
-  let sig = sig_ots ++ authpath in
-  sig.
-
-(**********************************************************************************************************************)
+(**************************************************************************************************)
 
 module type SignatureScheme = {
     proc kg() : keypair
     proc sign(sk : sk_t, m : msg_t) : sig_t * sk_t
     proc verify(pk : pk_t, m : msg_t, s : sig_t) : bool
-}.
-
-(*123*)
-op nbytes_radndom : nbytes.
-
-module XMSS : SignatureScheme = {
-  proc kg() : keypair = {
-    var idx : W32.t;
-    var i : int <- 0;
-    var pk : pk_t;
-    var sk : sk_t;
-    var wots_skey : wots_sk list;
-    var wots_sk_i : wots_sk;
-    var sk_prf : nbytes;
-    var _seed : seed;
-    var root : nbytes;
-    var address : adrs;
-
-    while (i < 2^h) {
-      wots_sk_i <@ WOTS.genSK();
-      wots_skey <- put wots_skey i wots_sk_i;
-      i <- i + 1;
-    }
-
-    sk_prf <- nbytes_radndom;
-    _seed <- nbytes_radndom;
-    address <- zero_address;
-    root <@ Treehash.treehash(sk, 0, h, address);
-
-    (* Check if this is ok *)
-    sk <- (oid, idx, _seed, sk_prf, _seed, root);
-    pk <- (oid, root, _seed);
-
-    return (pk, sk);
-  }
-
-  proc sign(sk : sk_t, m : msg_t) : sig_t * sk_t = {
-    var sig : sig_t <- witness;
-    
-    var idx_sig : W32.t;
-
-    var address : adrs <- zero_address;
-
-    idx_sig <- sk.`2;
-
-    return (sig, sk);
-  }
-
-  proc verify(pk : pk_t, m : msg_t, s : sig_t) : bool = {
-    var is_valid : bool <- false;
-
-    return is_valid;
-  }
 }.
